updating

locallyNameless/NonSpec.v
@@ -5,29 +5,56 @@ Require Import sets.
 
 Definition pHeap := heap pivar_state. 
 
-Definition pctxt := ptrm -> ptrm.
+Inductive pctxt : Type :=
+|pbindCtxt : pctxt -> ptrm -> pctxt
+|phandleCtxt : pctxt -> ptrm -> pctxt 
+|pholeCtxt : pctxt.
 
 Fixpoint pdecompose (t:ptrm) : (pctxt * ptrm) :=
   match t with
       |pbind M N => let (E, M') := pdecompose M
-                    in (fun x => pbind (E x) N, M')
+                    in (pbindCtxt E N, M')
       |phandle M N => let (E, M') := pdecompose M
-                      in (fun x => phandle (E x) N, M')
-      |_ => (fun x => x, t)
+                      in (phandleCtxt E N, M')
+      |_ => (pholeCtxt, t)
   end. 
 
+(*
+Fixpoint isPVal (t:ptrm) : bool :=
+  match t with
+      |pret N => true
+      |praise N => true
+      |_ => false
+  end. 
 
-Theorem pdecomposeEq : forall M E e, pdecompose M = (E, e) -> M = E e. 
+Fixpoint pdecompose (t:ptrm) : (pctxt * ptrm) :=
+  match t with
+      |pbind M N => if isPVal M
+                    then (pholeCtxt, pbind M N)
+                    else let (E, M') := pdecompose M
+                         in (pbindCtxt E N, M')
+      |phandle M N => if isPVal M 
+
+                      then (pholeCtxt, phandle M N)
+                      else let (E, M') := pdecompose M
+                           in (phandleCtxt E N, M')
+      |_ => (pholeCtxt, t)
+  end. 
+*)
+
+Fixpoint pfill (c:pctxt) (t:ptrm) : ptrm :=
+  match c with
+      |pbindCtxt E N => pbind (pfill E t) N
+      |phandleCtxt E N => phandle (pfill E t) N
+      |pholeCtxt => t
+  end. 
+
+Theorem pdecomposeEq : forall M E e, pdecompose M = (E, e) -> M = pfill E e. 
 Proof.
-  induction M; intros; simpl in *; inversion H; try reflexivity. 
-  {destruct (pdecompose M1). inversion H; inversion H1; subst. 
-   assert((p,e)=(p,e)) by reflexivity. apply IHM1 in H0. subst. 
-   reflexivity. }
-  {destruct (pdecompose M1). inversion H; inversion H1; subst. 
-   assert((p,e)=(p,e)) by reflexivity. apply IHM1 in H0. subst. 
-   reflexivity. }
+  induction M; intros; simpl in *; inversion H; try reflexivity; try solve[
+  destruct (pdecompose M1); inversion H; inversion H1; subst;  
+   assert((p,e)=(p,e)) by reflexivity; apply IHM1 in H0; subst; reflexivity]. 
 Qed. 
-
 
 Definition pPool := Ensemble ptrm. 
 Definition pSingleton := Singleton ptrm. 
@@ -35,30 +62,30 @@ Definition pUnion := Union ptrm.
 
 Inductive pstep : pHeap -> pPool -> pPool -> pHeap -> pPool -> pPool -> Prop :=
 |PBind : forall E t M N h T, 
-           pterm t -> pdecompose t = (E, pbind (pret M) N) -> 
-           pstep h T (pSingleton t) h T (pSingleton(E(papp N M)))
+            pdecompose t = (pbindCtxt E N, pret M) -> 
+           pstep h T (pSingleton t) h T (pSingleton(pfill E(papp N M)))
 |PBindRaise : forall E t M N h T,
-                pterm t -> pdecompose t = (E, pbind (praise M) N) -> 
-                pstep h T (pSingleton t) h T (pSingleton (E(praise M)))
+                 pdecompose t = (pbindCtxt E N, praise M) -> 
+                pstep h T (pSingleton t) h T (pSingleton (pfill E(praise M)))
 |pHandle : forall E t M N h T,
-             pterm t -> pdecompose t = (E, phandle (praise M) N) -> 
-             pstep h T (pSingleton t) h T (pSingleton (E(papp N M)))
+              pdecompose t = (phandleCtxt E N, praise M) -> 
+             pstep h T (pSingleton t) h T (pSingleton (pfill E(papp N M)))
 |pHandleRet : forall E t M N h T,
-                pterm t -> pdecompose t = (E, phandle (pret M) N) -> 
-                pstep h T (pSingleton t) h T (pSingleton (E(pret M)))
+                 pdecompose t = (phandleCtxt E N, pret M) -> 
+                pstep h T (pSingleton t) h T (pSingleton (pfill E(pret M)))
 |pFork : forall E t M h T,
-           pterm t -> pdecompose t = (E, pfork M) -> 
-           pstep h T (pSingleton t) h (Add ptrm T M) (pSingleton (E(pret punit)))
+            pdecompose t = (E, pfork M) -> 
+           pstep h T (pSingleton t) h T (Couple ptrm (pfill E(pret punit)) M)
 |PGet : forall E M t h T x,
-          pterm t -> heap_lookup x h = Some(pfull M) -> pdecompose t = (E, pget (pfvar x)) -> 
-          pstep h T (pSingleton t) h T (pSingleton (E(pret M)))
-|PPut : forall E t M h h' T x y,
-          pterm t -> pdecompose t = (E, pput (pfvar x) M) -> heap_lookup x h = Some pempty ->
+           heap_lookup x h = Some(pfull M) -> pdecompose t = (E, pget (pfvar x)) -> 
+          pstep h T (pSingleton t) h T (pSingleton (pfill E(pret M)))
+|PPut : forall E t M h h' T x,
+           pdecompose t = (E, pput (pfvar x) M) -> heap_lookup x h = Some pempty ->
           h' = replace x (pfull M) h ->
-          pstep h T (pSingleton t) (replace y (pfull M) h) T (pSingleton (E (pret punit)))
+          pstep h T (pSingleton t) (replace x (pfull M) h) T (pSingleton (pfill E (pret punit)))
 |PNew : forall E t h h' T x,
              pdecompose t = (E, pnew) -> (x, h') = extend pempty h ->
-             pstep h T (pSingleton t) h' T (pSingleton (E (pret (pfvar x))))
+             pstep h T (pSingleton t) h' T (pSingleton (pfill E (pret (pfvar x))))
 |PTerminate : forall h T M, pstep h T (pSingleton (pret M)) h T (Empty_set ptrm)
                 
 .
